fixtures/TypeChecker.mli
@@ -1475,6 +1475,12 @@ val check_fn_root_shadow_generic_direct_store_safe_summary :
 val check_fn_root_shadow_direct_receiver_method_store_safe_summary :
   global_env -> fn_def -> bool
 
+val check_fn_root_shadow_synthetic_direct_call_ready_summary :
+  global_env -> fn_def -> bool
+
+val check_env_root_shadow_synthetic_direct_call_ready_summary :
+  global_env -> bool
+
 val check_fn_root_shadow_no_capture_direct_call_component_store_safe_summary :
   global_env -> fn_def -> bool
 
@@ -1606,6 +1612,9 @@ val check_env_end2end_direct_receiver_mixed_ready : global_env -> bool
 
 val check_env_end2end_direct_receiver_absent_mixed_ready : global_env -> bool
 
+val check_env_end2end_direct_receiver_synthetic_mixed_ready :
+  global_env -> bool
+
 val infer_program_env_end2end_strict_exact_closure_direct_receiver :
   global_env -> global_env infer_result
 
@@ -1627,6 +1636,12 @@ val infer_program_env_end2end_assoc_direct_receiver_absent_mixed :
   global_env -> global_env infer_result
 
 val check_program_env_end2end_assoc_direct_receiver_absent_mixed :
+  global_env -> bool
+
+val infer_program_env_end2end_assoc_direct_receiver_synthetic_mixed :
+  global_env -> global_env infer_result
+
+val check_program_env_end2end_assoc_direct_receiver_synthetic_mixed :
   global_env -> bool
 
 val infer_program_env_end2end_assoc_strict_exact_closure_direct_receiver_mixed :
